Reclaim `coq_session_client.v`

src/program_proof/session/definitions.v
@@ -15,13 +15,19 @@ Proof.
   reflexivity.
 Qed.
 
-#[global] Opaque CONSTANT.
-
-Definition nat_ge_CONSTANT (n : nat) : Prop :=
+Definition nat_le_CONSTANT (n : nat) : Prop :=
   Z.of_nat n <= CONSTANT.
 
-Definition u64_ge_CONSTANT (u : u64) : Prop :=
+Definition u64_le_CONSTANT (u : u64) : Prop :=
   uint.Z u <= CONSTANT.
+
+Lemma CONSTANT_ge_0
+  : u64_le_CONSTANT (W64 0).
+Proof.
+  red; unfold CONSTANT. word.
+Qed.
+
+#[global] Opaque CONSTANT.
 
 Module Operation.
 
@@ -234,7 +240,7 @@ Section heap.
     refine (
       {|
         into_val.to_val := client_val;
-        from_val := client_from_val ;
+        from_val := client_from_val;
         IntoVal_def := (W64 0, W64 0, IntoVal_def Slice.t, IntoVal_def Slice.t, W64 0);
       |}
     ).
@@ -248,60 +254,60 @@ Section heap.
 
   Definition is_operation (opv: Slice.t*u64) (op: Operation.t) (len_opv: nat) : iProp Σ :=
     ⌜opv.2 = op.(Operation.Data)⌝ ∗
-    ⌜len_opv = length op.(Operation.VersionVector) /\ Forall u64_ge_CONSTANT op.(Operation.VersionVector)⌝ ∗
+    ⌜len_opv = length op.(Operation.VersionVector) /\ Forall u64_le_CONSTANT op.(Operation.VersionVector)⌝ ∗
     own_slice_small opv.1 uint64T DfracDiscarded op.(Operation.VersionVector).
 
   Definition operation_slice (s: Slice.t) (l: list Operation.t) (n: nat) : iProp Σ :=
     ∃ ops, own_slice s (struct.t Operation) (DfracOwn 1) ops ∗ [∗ list] opv;o ∈ ops;l, is_operation opv o n.
 
   Definition is_message (msgv: tuple_of [u64,u64,u64,u64,u64,Slice.t,u64,u64,Slice.t,u64,u64,u64,u64,u64,u64,Slice.t,u64,u64]) (msg: Message.t) (n: nat) (len_c2s: nat) (len_s2c: nat) : iProp Σ :=
-    ⌜msgv!(0) = msg.(Message.MessageType) /\ u64_ge_CONSTANT msg.(Message.MessageType)⌝ ∗
-    ⌜msgv!(1) = msg.(Message.C2S_Client_Id) /\ u64_ge_CONSTANT msg.(Message.C2S_Client_Id)⌝ ∗
-    ⌜msgv!(2) = msg.(Message.C2S_Server_Id) /\ u64_ge_CONSTANT msg.(Message.C2S_Server_Id)⌝ ∗
-    ⌜msgv!(3) = msg.(Message.C2S_Client_OperationType) /\ u64_ge_CONSTANT msg.(Message.C2S_Client_OperationType)⌝ ∗
+    ⌜msgv!(0) = msg.(Message.MessageType) /\ u64_le_CONSTANT msg.(Message.MessageType)⌝ ∗
+    ⌜msgv!(1) = msg.(Message.C2S_Client_Id) /\ u64_le_CONSTANT msg.(Message.C2S_Client_Id)⌝ ∗
+    ⌜msgv!(2) = msg.(Message.C2S_Server_Id) /\ u64_le_CONSTANT msg.(Message.C2S_Server_Id)⌝ ∗
+    ⌜msgv!(3) = msg.(Message.C2S_Client_OperationType) /\ u64_le_CONSTANT msg.(Message.C2S_Client_OperationType)⌝ ∗
     ⌜msgv!(4) = msg.(Message.C2S_Client_Data)⌝ ∗
     own_slice_small msgv!(5) uint64T (DfracOwn 1) msg.(Message.C2S_Client_VersionVector) ∗
-    ⌜len_c2s = length msg.(Message.C2S_Client_VersionVector) /\ Forall u64_ge_CONSTANT msg.(Message.C2S_Client_VersionVector)⌝ ∗
-    ⌜msgv!(6) = msg.(Message.S2S_Gossip_Sending_ServerId) /\ u64_ge_CONSTANT msg.(Message.S2S_Gossip_Sending_ServerId)⌝ ∗
-    ⌜msgv!(7) = msg.(Message.S2S_Gossip_Receiving_ServerId) /\ u64_ge_CONSTANT msg.(Message.S2S_Gossip_Receiving_ServerId)⌝ ∗
+    ⌜len_c2s = length msg.(Message.C2S_Client_VersionVector) /\ Forall u64_le_CONSTANT msg.(Message.C2S_Client_VersionVector)⌝ ∗
+    ⌜msgv!(6) = msg.(Message.S2S_Gossip_Sending_ServerId) /\ u64_le_CONSTANT msg.(Message.S2S_Gossip_Sending_ServerId)⌝ ∗
+    ⌜msgv!(7) = msg.(Message.S2S_Gossip_Receiving_ServerId) /\ u64_le_CONSTANT msg.(Message.S2S_Gossip_Receiving_ServerId)⌝ ∗
     operation_slice msgv!(8) msg.(Message.S2S_Gossip_Operations) n ∗
-    ⌜msgv!(9) = msg.(Message.S2S_Gossip_Index) /\ u64_ge_CONSTANT msg.(Message.S2S_Gossip_Index)⌝ ∗
-    ⌜msgv!(10) = msg.(Message.S2S_Acknowledge_Gossip_Sending_ServerId) /\ u64_ge_CONSTANT msg.(Message.S2S_Acknowledge_Gossip_Sending_ServerId)⌝ ∗
-    ⌜msgv!(11) = msg.(Message.S2S_Acknowledge_Gossip_Receiving_ServerId) /\ u64_ge_CONSTANT msg.(Message.S2S_Acknowledge_Gossip_Receiving_ServerId)⌝ ∗
-    ⌜msgv!(12) = msg.(Message.S2S_Acknowledge_Gossip_Index) /\ u64_ge_CONSTANT msg.(Message.S2S_Acknowledge_Gossip_Index)⌝ ∗
-    ⌜msgv!(13) = msg.(Message.S2C_Client_OperationType) /\ u64_ge_CONSTANT msg.(Message.S2C_Client_OperationType)⌝ ∗
+    ⌜msgv!(9) = msg.(Message.S2S_Gossip_Index) /\ u64_le_CONSTANT msg.(Message.S2S_Gossip_Index)⌝ ∗
+    ⌜msgv!(10) = msg.(Message.S2S_Acknowledge_Gossip_Sending_ServerId) /\ u64_le_CONSTANT msg.(Message.S2S_Acknowledge_Gossip_Sending_ServerId)⌝ ∗
+    ⌜msgv!(11) = msg.(Message.S2S_Acknowledge_Gossip_Receiving_ServerId) /\ u64_le_CONSTANT msg.(Message.S2S_Acknowledge_Gossip_Receiving_ServerId)⌝ ∗
+    ⌜msgv!(12) = msg.(Message.S2S_Acknowledge_Gossip_Index) /\ u64_le_CONSTANT msg.(Message.S2S_Acknowledge_Gossip_Index)⌝ ∗
+    ⌜msgv!(13) = msg.(Message.S2C_Client_OperationType) /\ u64_le_CONSTANT msg.(Message.S2C_Client_OperationType)⌝ ∗
     ⌜msgv!(14) = msg.(Message.S2C_Client_Data)⌝ ∗
     own_slice_small msgv!(15) uint64T (DfracOwn 1) msg.(Message.S2C_Client_VersionVector) ∗
-    ⌜len_s2c = length msg.(Message.S2C_Client_VersionVector) /\ Forall u64_ge_CONSTANT msg.(Message.S2C_Client_VersionVector)⌝ ∗
-    ⌜msgv!(16) = msg.(Message.S2C_Server_Id) /\ u64_ge_CONSTANT msg.(Message.S2C_Server_Id)⌝ ∗
-    ⌜msgv!(17) = msg.(Message.S2C_Client_Number) /\ u64_ge_CONSTANT msg.(Message.S2C_Server_Id)⌝.
+    ⌜len_s2c = length msg.(Message.S2C_Client_VersionVector) /\ Forall u64_le_CONSTANT msg.(Message.S2C_Client_VersionVector)⌝ ∗
+    ⌜msgv!(16) = msg.(Message.S2C_Server_Id) /\ u64_le_CONSTANT msg.(Message.S2C_Server_Id)⌝ ∗
+    ⌜msgv!(17) = msg.(Message.S2C_Client_Number) /\ u64_le_CONSTANT msg.(Message.S2C_Server_Id)⌝.
 
   Definition message_slice (s: Slice.t) (l: list Message.t) (n: nat) (len_c2s: nat) : iProp Σ :=
     ∃ msgs, own_slice s (struct.t server.Message) (DfracOwn 1) msgs ∗ [∗ list] mv;m ∈ msgs;l, ∃ len_s2c, is_message mv m n len_c2s len_s2c.
 
   Definition is_server' (sv: tuple_of [u64,u64,Slice.t,Slice.t,Slice.t,Slice.t,Slice.t,Slice.t]) (s: Server.t) (n: nat) (len_vc: nat) (len_op: nat) (len_mo: nat) (len_po: nat) (len_ga: nat) (OWN_UnsatisfiedRequests: bool) : iProp Σ :=
-    ⌜sv!(0) = s.(Server.Id) /\ u64_ge_CONSTANT s.(Server.Id)⌝ ∗
-    ⌜sv!(1) = s.(Server.NumberOfServers) /\ u64_ge_CONSTANT s.(Server.NumberOfServers)⌝ ∗
+    ⌜sv!(0) = s.(Server.Id) /\ u64_le_CONSTANT s.(Server.Id)⌝ ∗
+    ⌜sv!(1) = s.(Server.NumberOfServers) /\ u64_le_CONSTANT s.(Server.NumberOfServers)⌝ ∗
     (if OWN_UnsatisfiedRequests then message_slice sv!(2) s.(Server.UnsatisfiedRequests) n len_vc else emp)%I ∗
     own_slice_small sv!(3) uint64T (DfracOwn 1) s.(Server.VectorClock) ∗
-    ⌜len_vc = length s.(Server.VectorClock) /\ Forall u64_ge_CONSTANT s.(Server.VectorClock)⌝ ∗
+    ⌜len_vc = length s.(Server.VectorClock) /\ Forall u64_le_CONSTANT s.(Server.VectorClock)⌝ ∗
     operation_slice sv!(4) s.(Server.OperationsPerformed) len_op ∗
     operation_slice sv!(5) s.(Server.MyOperations) len_mo ∗
     operation_slice sv!(6) s.(Server.PendingOperations) len_po ∗
     own_slice_small sv!(7) uint64T (DfracOwn 1) s.(Server.GossipAcknowledgements) ∗
-    ⌜len_ga = length s.(Server.GossipAcknowledgements) /\ Forall u64_ge_CONSTANT s.(Server.GossipAcknowledgements)⌝.
+    ⌜len_ga = length s.(Server.GossipAcknowledgements) /\ Forall u64_le_CONSTANT s.(Server.GossipAcknowledgements)⌝.
 
   Definition is_server sv s n len_vc len_op len_mo len_po len_ga : iProp Σ :=
     is_server' sv s n len_vc len_op len_mo len_po len_ga true.
 
   Definition is_client (cv: tuple_of [u64,u64,Slice.t,Slice.t,u64]) (c: Client.t) (n: nat) : iProp Σ :=
-    ⌜cv!(0) = c.(Client.Id) /\ u64_ge_CONSTANT c.(Client.Id)⌝ ∗
-    ⌜cv!(1) = c.(Client.NumberOfServers) /\ u64_ge_CONSTANT c.(Client.NumberOfServers)⌝ ∗
+    ⌜cv!(0) = c.(Client.Id) /\ u64_le_CONSTANT c.(Client.Id)⌝ ∗
+    ⌜cv!(1) = c.(Client.NumberOfServers) /\ u64_le_CONSTANT c.(Client.NumberOfServers)⌝ ∗
     ⌜n = uint.nat c.(Client.NumberOfServers)⌝ ∗
     own_slice_small cv!(2) uint64T (DfracOwn 1) c.(Client.WriteVersionVector) ∗
-    ⌜n = length c.(Client.WriteVersionVector) /\ Forall u64_ge_CONSTANT c.(Client.WriteVersionVector)⌝ ∗
+    ⌜n = length c.(Client.WriteVersionVector) /\ Forall u64_le_CONSTANT c.(Client.WriteVersionVector)⌝ ∗
     own_slice_small cv!(3) uint64T (DfracOwn 1) c.(Client.ReadVersionVector) ∗
-    ⌜n = length c.(Client.ReadVersionVector) /\ Forall u64_ge_CONSTANT c.(Client.ReadVersionVector)⌝ ∗
+    ⌜n = length c.(Client.ReadVersionVector) /\ Forall u64_le_CONSTANT c.(Client.ReadVersionVector)⌝ ∗
     ⌜cv!(4) = c.(Client.SessionSemantic)⌝.
 
 End heap.
