src/program_proof/session/gossip.v
@@ -213,7 +213,7 @@ Section heap.
         ⌜WEAK_SERVER_INVARIANT (fun _s => _s.(Server.Id) = Id /\ _s.(Server.NumberOfServers) = NumberOfServers /\ _s.(Server.UnsatisfiedRequests) = UnsatisfiedRequests /\ _s.(Server.MyOperations) = MyOperations /\ _s.(Server.GossipAcknowledgements) = GossipAcknowledgements) (coq_receiveGossip s msg)⌝
     }}}.
   Proof.
-    (* set ((fun _s => _s.(Server.Id) = Id /\ _s.(Server.NumberOfServers) = NumberOfServers /\ _s.(Server.UnsatisfiedRequests) = UnsatisfiedRequests /\ _s.(Server.MyOperations) = MyOperations /\ _s.(Server.GossipAcknowledgements) = GossipAcknowledgements)) as EXTRA_s.
+    (* set (fun _s => _s.(Server.Id) = Id /\ _s.(Server.NumberOfServers) = NumberOfServers /\ _s.(Server.UnsatisfiedRequests) = UnsatisfiedRequests /\ _s.(Server.MyOperations) = MyOperations /\ _s.(Server.GossipAcknowledgements) = GossipAcknowledgements) as EXTRA_s.
     rewrite redefine_server_val redefine_message_val. TypeVector.des sv. TypeVector.des msgv. iIntros "%Φ (H_server & H_message & %H_invariant) HΦ". destruct H_invariant; destruct EXTRA_SERVER_INVARIANT as (<- & <- & <- & <- & <-).
     iDestruct "H_server" as "(%H1 & %H2 & H3 & H4 & %H5 & H6 & H7 & H8 & H9 & %H10)". iDestruct "H_message" as "(%H11 & %H12 & %H13 & %H14 & %H15 & H16 & %H17 & %H18 & %H19 & H20 & %H21 & %H22 & %H23 & %H24 & %H25 & %H26 & H27 & %H28 & %H29 & %H30)".
     rewrite /receiveGossip; simplNotation; subst.
